abts! hard to define LR now :(

f.v
@@ -1,528 +1,59 @@
 Require Import util.
+Require Import abt.
+
+Module tyop.
+  Inductive t' :=
+  | arrow
+  | all
+  .
+  Definition t := t'.
+
+  Definition arity (op : t) : arity.t :=
+    match op with
+    | arrow => [0; 0]
+    | all => [1]
+    end.
+
+  Definition eq_dec : forall x y : t, {x = y} + {x <> y}.
+    decide equality.
+  Defined.
+
+End tyop.
+
+Module exprop.
+  Inductive t' :=
+  | abs
+  | app
+  | tyabs
+  | tyapp
+  .
+  Definition t := t'.
+
+  Definition arity (op : t) : arity.t :=
+    match op with
+    | abs => [1]
+    | app => [0; 0]
+    | tyabs => [0]
+    | tyapp => [0]
+    end.
+
+  Definition eq_dec : forall x y : t, {x = y} + {x <> y}.
+    decide equality.
+  Defined.
+End exprop.
 
 Module type.
-  Inductive t :=
-  | var (alpha : nat) : t
-  | arrow : t -> t -> t
-  | all : t -> t
-  .
-
-  Fixpoint wf (n : nat) (ty : t) :=
-    match ty with
-    | var a => a < n
-    | arrow ty1 ty2 => wf n ty1 /\ wf n ty2
-    | all ty' => wf (S n) ty'
-    end.
-
-  Fixpoint shift (c d : nat) (ty : t) : t :=
-    match ty with
-    | var a => var (if a <? c then a else d + a)
-    | arrow ty1 ty2 => arrow (shift c d ty1) (shift c d ty2)
-    | all ty' => all (shift (S c) d ty')
-    end.
-
-  Fixpoint identity_subst (n : nat) : list type.t :=
-    match n with
-    | 0 => []
-    | S n => var 0 :: List.map (shift 0 1) (identity_subst n)
-    end.
-
-  Lemma identity_subst_length : forall n, length (identity_subst n) = n.
-  Proof.
-    induction n; simpl.
-    - auto.
-    - rewrite map_length. auto using f_equal.
-  Qed.
-
-  Lemma shift_shift :
-    forall ty c1 d1 c2 d2,
-      c2 <= c1 ->
-      shift c2 d2 (shift c1 d1 ty) =
-      shift (c1 + d2) d1 (shift c2 d2 ty).
-  Proof.
-    induction ty; intros c1 d1 c2 d2 LT; simpl.
-    - f_equal.
-      repeat match goal with
-      | [  |- context [ ?x <? ?y ] ] =>
-        destruct (Nat.ltb_spec x y)
-      end; omega.
-    - f_equal; eauto.
-    - f_equal. now rewrite IHty by omega.
-  Qed.
-
-  Fixpoint subst (D : list t) (ty : t) : t :=
-    match ty with
-    | var a => match List.nth_error D a with
-              | Some ty' => ty'
-              | None => ty
-              end
-    | arrow ty1 ty2 => arrow (subst D ty1) (subst D ty2)
-    | all ty' => all (subst (var 0 :: map (shift 0 1) D) ty')
-    end.
-
-  Lemma shift_subst :
-    forall ty c d D,
-      wf (List.length D) ty ->
-      shift c d (subst D ty) =
-      subst (List.map (shift c d) D) ty.
-  Proof.
-    induction ty; intros c d D WF.
-    - simpl in *.
-      rewrite nth_error_map.
-      destruct (nth_error D alpha) eqn:?.
-      + reflexivity.
-      + pose proof nth_error_Some D alpha.
-        intuition.
-    - simpl in *. f_equal; intuition.
-    - simpl. f_equal.
-      rewrite IHty by (simpl; rewrite map_length; assumption).
-      simpl.
-      f_equal. f_equal.
-      rewrite !map_map.
-      apply map_ext.
-      intros ty'.
-      rewrite shift_shift with (c2 := 0) by omega.
-      f_equal. omega.
-  Qed.
-
-  Lemma subst_shift :
-    forall ty D1 D2 D3,
-      wf (List.length (D1 ++ D3)) ty ->
-      subst (D1 ++ D2 ++ D3) (shift (List.length D1) (List.length D2) ty) =
-      subst (D1 ++ D3) ty.
-  Proof.
-    induction ty; simpl; intros D1 D2 D3 H.
-    - destruct (Nat.ltb_spec alpha (length D1)).
-      + now rewrite !nth_error_app1 by assumption.
-      + rewrite !nth_error_app2 by omega.
-        rewrite plus_comm.
-        rewrite Nat.add_sub_swap by assumption.
-        rewrite <- Nat.add_sub_assoc by omega.
-        rewrite Nat.sub_diag.
-        rewrite Nat.add_0_r.
-        break_match; auto.
-        pose proof nth_error_Some D3 (alpha - length D1).
-        rewrite !app_length in *.
-        now intuition.
-    - f_equal; intuition.
-    - f_equal.
-      rewrite !map_app.
-      rewrite !app_comm_cons.
-      erewrite <- IHty.
-      + f_equal. simpl.
-        now rewrite !map_length.
-      + simpl. now rewrite app_length, !map_length in *.
-  Qed.
-
-  Lemma wf_shift :
-    forall ty c d n,
-      wf n ty ->
-      wf (d + n) (shift c d ty).
-  Proof.
-    induction ty; simpl; intros c d m H.
-    - destruct (Nat.ltb_spec alpha c); omega.
-    - intuition.
-    - rewrite plus_n_Sm. auto.
-  Qed.
-
-  Lemma subst_subst :
-    forall ty D1 D2,
-      wf (List.length D1) ty ->
-      List.Forall (wf (List.length D2)) D1 ->
-      subst D2 (subst D1 ty) =
-      subst (List.map (subst D2) D1) ty.
-  Proof.
-    induction ty; intros D1 D2 WF F.
-    - cbn [subst].
-      cbn [wf] in WF.
-      pose proof nth_error_Some D1 alpha.
-      rewrite nth_error_map.
-      destruct (nth_error D1 alpha) eqn:TY; intuition congruence.
-    - simpl in *.
-      intuition.
-      now rewrite IHty1, IHty2 by auto.
-    - cbn [subst].
-      erewrite IHty.
-      + f_equal. f_equal.
-        simpl. f_equal.
-        rewrite !map_map.
-        apply map_ext_in.
-        intros ty' I.
-        assert (wf (length D2) ty') by (eapply Forall_forall; eauto).
-        rewrite shift_subst by assumption.
-        apply subst_shift with (D1 := []) (D2 := [var 0]).
-        simpl.
-        now rewrite map_length.
-      + simpl.
-        now rewrite map_length.
-      + simpl. constructor.
-        * rewrite map_length. simpl. omega.
-        * rewrite map_length.
-          rewrite Forall_map.
-          eapply Forall_impl; [|eauto].
-          intros ty' H.
-          apply wf_shift with (d := 1); auto.
-  Qed.
-
-  Lemma wf_subst :
-    forall ty n D,
-      wf (length D) ty ->
-      List.Forall (wf n) D ->
-      wf n (subst D ty).
-  Proof.
-    induction ty; simpl; intros x D WF F.
-    - break_match.
-      + now eapply Forall_nth; eauto.
-      + pose proof nth_error_Some D alpha.
-        intuition.
-    - intuition eauto.
-    - eapply IHty; eauto.
-      + simpl. now rewrite map_length.
-      + constructor.
-        * simpl. omega.
-        * rewrite Forall_map.
-          eapply Forall_impl; [|eauto].
-          intros.
-          now apply wf_shift with (d := 1).
-  Qed.
-
-  Lemma nth_error_identity_subst :
-    forall n x y,
-      nth_error (identity_subst n) x = Some y ->
-      y = var x.
-  Proof.
-    induction n; intros x y NE; destruct x; simpl in *; try congruence.
-    rewrite nth_error_map in NE.
-    break_match; try discriminate.
-    apply IHn in Heqo.
-    subst. simpl in *. congruence.
-  Qed.
-
-  Lemma subst_identity :
-    forall e n,
-      subst (identity_subst n) e = e.
-  Proof.
-    induction e as [x| |]; intros n; cbn [subst].
-    - destruct (nth_error (identity_subst n) x) eqn:E; auto.
-      now apply nth_error_identity_subst in E.
-    - now f_equal; auto.
-    - f_equal.
-      now apply IHe with (n := (S n)).
-  Qed.
-
-  Lemma subst_empty :
-    forall e,
-      subst [] e = e.
-  Proof.
-    intros e.
-    exact (subst_identity e 0).
-  Qed.
-
-  Lemma wf_weaken :
-    forall ty n d,
-      n <= d ->
-      wf n ty ->
-      wf d ty.
-  Proof.
-    induction ty; simpl; intros n d WF; intuition eauto with arith.
-  Qed.
-
-  Lemma shift_nop :
-    forall ty c d n,
-      n <= c ->
-      wf n ty ->
-      shift c d ty = ty.
-  Proof.
-    induction ty; simpl; intros c d n LE WF; f_equal; intuition eauto.
-    - destruct (Nat.ltb_spec alpha c); omega.
-    - eapply IHty; [|eauto]. omega.
-  Qed.
-
-  Lemma shift_nop_d :
-    forall ty c,
-      shift c 0 ty = ty.
-  Proof.
-    induction ty; intros c; simpl; f_equal; auto.
-    break_match; auto.
-  Qed.
-
-  Lemma identity_subst_wf :
-    forall n,
-      Forall (wf n) (identity_subst n).
-  Proof.
-    induction n; simpl; constructor.
-    - simpl. omega.
-    - rewrite Forall_map. eapply Forall_impl; [|apply IHn].
-      intros ty WF.
-      now apply wf_shift with (c := 0) (d := 1).
-  Qed.
-
-  Lemma shift_merge :
-    forall e c d1 d2,
-      shift c d2 (shift c d1 e) = shift c (d2 + d1) e.
-  Proof.
-    induction e; intros c d1 d2; simpl.
-    - destruct (Nat.ltb_spec alpha c).
-      + destruct (Nat.ltb_spec alpha c); [reflexivity|omega].
-      + destruct (Nat.ltb_spec (d1 + alpha) c); f_equal; omega.
-    - f_equal; auto.
-    - f_equal. auto.
-  Qed.
+   Include abt.abt tyop.
+   Notation arrow ty1 ty2 := (op tyop.arrow [bind 0 ty1; bind 0 ty2]).
+   Notation all ty := (op tyop.all [bind 1 ty]).
 End type.
 
 Module expr.
-  Inductive t :=
-  | var (x : nat) : t
-  | abs : t -> t
-  | app : t -> t -> t
-  | tyabs : t -> t
-  | tyapp : t -> t
-  .
-
-  Fixpoint wf (n : nat) (e : t) :=
-    match e with
-    | var x => x < n
-    | abs e' => wf (S n) e'
-    | app e1 e2 => wf n e1 /\ wf n e2
-    | tyabs e' => wf n e'
-    | tyapp e' => wf n e'
-    end.
-
-  Fixpoint shift (c d : nat) (e : t) : t :=
-    match e with
-    | var x => var (if x <? c then x else d + x)
-    | abs e' => abs (shift (S c) d e')
-    | app e1 e2 => app (shift c d e1) (shift c d e2)
-    | tyabs e' => tyabs (shift c d e')
-    | tyapp e' => tyapp (shift c d e')
-    end.
-
-  Fixpoint subst (rho : list expr.t) (e : t) : t :=
-    match e with
-    | var x => match nth_error rho x with
-              | Some e' => e'
-              | None => e
-              end
-    | abs e' => abs (subst (var 0 :: List.map (shift 0 1) rho) e')
-    | app e1 e2 => app (subst rho e1) (subst rho e2)
-    | tyabs e' => tyabs (subst rho e')
-    | tyapp e' => tyapp (subst rho e')
-    end.
-
-  Fixpoint identity_subst (n : nat) : list expr.t :=
-    match n with
-    | 0 => []
-    | S n => var 0 :: List.map (shift 0 1) (identity_subst n)
-    end.
-
-  Lemma identity_subst_length : forall n, length (identity_subst n) = n.
-  Proof.
-    induction n; simpl.
-    - auto.
-    - rewrite map_length. auto using f_equal.
-  Qed.
-
-  Lemma wf_shift :
-    forall e c d n,
-      wf n e ->
-      wf (d + n) (shift c d e).
-  Proof.
-    induction e; simpl; intros c d m H.
-    - destruct (Nat.ltb_spec x c); omega.
-    - rewrite plus_n_Sm. auto.
-    - intuition.
-    - auto.
-    - auto.
-  Qed.
-
-  Lemma wf_subst :
-    forall e n rho,
-      wf (length rho) e ->
-      Forall (wf n) rho ->
-      wf n (subst rho e).
-  Proof.
-    induction e; simpl; intros n rho WF F.
-    - break_match.
-      + now eapply Forall_nth; eauto.
-      + pose proof nth_error_Some rho x.
-        intuition.
-    - eapply IHe; eauto.
-      + simpl. now rewrite map_length.
-      + constructor.
-        * simpl. omega.
-        * rewrite Forall_map.
-          eapply Forall_impl; [|eauto].
-          intros.
-          now apply wf_shift with (d := 1).
-    - intuition eauto.
-    - apply IHe; auto.
-    - auto.
-  Qed.
-
-  Lemma shift_shift :
-    forall e c1 d1 c2 d2,
-      c2 <= c1 ->
-      shift c2 d2 (shift c1 d1 e) =
-      shift (c1 + d2) d1 (shift c2 d2 e).
-  Proof.
-    induction e; simpl; intros c1 d1 c2 d2 LT.
-    - f_equal.
-      repeat match goal with
-      | [  |- context [ ?x <? ?y ] ] =>
-        destruct (Nat.ltb_spec x y)
-      end; omega.
-    - f_equal. now rewrite IHe by omega.
-    - f_equal; eauto.
-    - f_equal. eauto.
-    - f_equal. eauto.
-  Qed.
-
-  Lemma shift_subst :
-    forall e c d rho,
-      wf (List.length rho) e ->
-      shift c d (subst rho e) =
-      subst (List.map (shift c d) rho) e.
-  Proof.
-    induction e; intros c d rho WF.
-    - simpl in *.
-      rewrite nth_error_map.
-      destruct (nth_error rho x) eqn:?.
-      + reflexivity.
-      + pose proof nth_error_Some rho x.
-        intuition.
-    - simpl. f_equal.
-      rewrite IHe by (simpl; rewrite map_length; assumption).
-      simpl.
-      f_equal. f_equal.
-      rewrite !map_map.
-      apply map_ext.
-      intros e'.
-      rewrite shift_shift with (c2 := 0) by omega.
-      f_equal. omega.
-    - simpl in *. f_equal; intuition.
-    - simpl in *. f_equal.
-      now rewrite IHe by assumption.
-    - simpl in *. f_equal.
-      auto.
-  Qed.
-
-  Lemma subst_shift :
-    forall e r1 r2 r3,
-      wf (List.length (r1 ++ r3)) e ->
-      subst (r1 ++ r2 ++ r3) (shift (List.length r1) (List.length r2) e) =
-      subst (r1 ++ r3) e.
-  Proof.
-    induction e; simpl; intros r1 r2 r3 WF; f_equal; intuition.
-    - destruct (Nat.ltb_spec x (length r1)).
-      + now rewrite !nth_error_app1 by assumption.
-      + rewrite !nth_error_app2 by omega.
-        rewrite plus_comm.
-        rewrite Nat.add_sub_swap by assumption.
-        rewrite <- Nat.add_sub_assoc by omega.
-        rewrite Nat.sub_diag.
-        rewrite Nat.add_0_r.
-        break_match; auto.
-        pose proof nth_error_Some r3 (x - length r1).
-        rewrite !app_length in *.
-        intuition.
-    - rewrite !map_app.
-      rewrite !app_comm_cons.
-      erewrite <- IHe.
-      + f_equal. simpl.
-        now rewrite !map_length.
-      + simpl. now rewrite app_length, !map_length in *.
-  Qed.
-
-  Lemma subst_subst :
-    forall e rho1 rho2,
-      wf (length rho1) e ->
-      Forall (wf (length rho2)) rho1 ->
-      subst rho2 (subst rho1 e) =
-      subst (List.map (subst rho2 ) rho1) e.
-  Proof.
-    induction e; simpl; intros rho1 rho2 WF F.
-    - rewrite nth_error_map.
-      break_match; auto.
-      pose proof nth_error_Some rho1 x.
-      intuition.
-    - f_equal. rewrite IHe.
-      + simpl.
-        f_equal. f_equal.
-        rewrite !map_map.
-        apply map_ext_in.
-        intros e' I.
-        pose proof subst_shift e' [] [var 0] (map (shift 0 1) rho2).
-        simpl in H.
-        assert (wf (length rho2) e') by (eapply Forall_forall; eauto).
-        rewrite H by now rewrite map_length.
-        now rewrite shift_subst by assumption.
-      + simpl. now rewrite map_length.
-      + simpl. rewrite map_length.
-        constructor.
-        * simpl. omega.
-        * rewrite Forall_map.
-          eapply Forall_impl; [| now eauto].
-          intros e' WF'.
-          now apply wf_shift with (d := 1).
-    - f_equal; intuition.
-    - f_equal; auto.
-    - f_equal; auto.
-  Qed.
-
-  Lemma nth_error_identity_subst :
-    forall n x y,
-      nth_error (identity_subst n) x = Some y ->
-      y = var x.
-  Proof.
-    induction n; intros x y NE; destruct x; simpl in *; try congruence.
-    rewrite nth_error_map in NE.
-    break_match; try discriminate.
-    apply IHn in Heqo.
-    subst. simpl in *. congruence.
-  Qed.
-
-  Lemma subst_identity :
-    forall e n,
-      subst (identity_subst n) e = e.
-  Proof.
-    induction e as [x| | | |]; intros n; cbn [subst].
-    - destruct (nth_error (identity_subst n) x) eqn:E; auto.
-      now apply nth_error_identity_subst in E.
-    - f_equal.
-      now apply IHe with (n := (S n)).
-    - now f_equal; auto.
-    - f_equal. auto.
-    - f_equal. auto.
-  Qed.
-
-  Lemma subst_empty :
-    forall e,
-      subst [] e = e.
-  Proof.
-    intros e.
-    exact (subst_identity e 0).
-  Qed.
-
-
-  Lemma subst_shift' :
-    forall e e' g,
-      wf (length g) e ->
-      subst (e' :: g) (shift 0 1 e) = subst g e.
-  Proof.
-    intros.
-    pose proof subst_shift e [] [e'] g.
-    auto.
-  Qed.
-
-  Lemma subst_shift_singleton :
-    forall e e',
-      wf 0 e ->
-      subst [e'] (shift 0 1 e) = e.
-  Proof.
-    intros.
-    rewrite subst_shift' by auto.
-    now rewrite subst_identity with (n := 0).
-  Qed.
+   Include abt.abt exprop.
+   Notation abs e := (op exprop.abs [bind 1 e]).
+   Notation app e1 e2 := (op exprop.app [bind 0 e1; bind 0 e2]).
+   Notation tyabs e := (op exprop.tyabs [bind 0 e]).
+   Notation tyapp e := (op exprop.tyapp [bind 0 e]).
 End expr.
 
 Module has_type.
@@ -565,7 +96,7 @@ Module has_type.
     - apply type.wf_subst.
       + simpl. now rewrite type.identity_subst_length.
       + constructor; auto.
-        clear H H0 H1 H2.
+        clear H H0 H1 H3 H4.
         induction n; simpl; constructor.
         * simpl. omega.
         * rewrite Forall_map.
