abt.v
@@ -1,0 +1,697 @@
+Require Import util.
+Set Implicit Arguments.
+
+Module valence.
+  Definition t : Type := nat.
+
+  Definition eq_dec : forall x y : t, {x = y} + {x <> y} := eq_nat_dec.
+End valence.
+
+Module arity.
+  Definition t : Type := list valence.t.
+
+  Definition eq_dec : forall x y : t, {x = y} + {x <> y}.
+    apply list_eq_dec.
+    apply valence.eq_dec.
+  Defined.
+End arity.
+
+Module Type OPERATOR.
+  Parameter t : Type.
+  Parameter eq_dec : forall x y : t, {x = y} + {x <> y}.
+  Parameter arity : t -> arity.t.
+End OPERATOR.
+
+Module abt (O : OPERATOR).
+  Local Unset Elimination Schemes.
+  Inductive t : Type :=
+  | var (x : nat) : t
+  | op : O.t -> list binder -> t
+  with
+  binder :=
+  | bind (s : nat) : t -> binder.
+
+  Section rect.
+    Variable P : t -> Type.
+    Variable Pb : binder -> Type.
+    Variable Pbl : list binder -> Type.
+
+    Hypotheses Pvar : forall x, P (var x).
+    Hypothesis Pop : forall o bs, Pbl bs -> P (op o bs).
+    Hypothesis Pbind : forall s e, P e -> Pb (bind s e).
+    Hypothesis Pblnil : Pbl [].
+    Hypothesis Pblcons : forall b bs, Pb b -> Pbl bs -> Pbl (b :: bs).
+
+    Fixpoint rect (e : t) : P e :=
+      let fix rect_list (l : list binder) : Pbl l :=
+          match l with
+          | [] => Pblnil
+          | b :: bs => Pblcons (rect_binder b) (rect_list bs)
+          end
+      in
+      match e with
+      | var x => Pvar x
+      | op o bs => Pop o (rect_list bs)
+      end
+    with rect_binder (b : binder) : Pb b :=
+      match b with
+      | bind s e => Pbind s (rect e)
+      end
+    .
+  End rect.
+
+  Section rect'.
+    Variable P : t -> Prop.
+    Variable Pb : binder -> Prop.
+    Let Pbl (bs : list binder) : Prop := Forall Pb bs.
+
+    Hypotheses Pvar : forall n, P (var n).
+    Hypothesis Pop : forall o bs, Pbl bs -> P (op o bs).
+    Hypothesis Pbind : forall n e, P e -> Pb (bind n e).
+
+    Definition rect' (e : t) : P e.
+      refine (rect P Pb Pbl Pvar Pop Pbind (Forall_nil _) _ e).
+      intros. constructor; auto.
+    Defined.
+  End rect'.
+
+
+  Fixpoint wf (n : nat) (e : t) :=
+    let fix go_list (n : nat) (bs : list binder) :=
+        match bs with
+        | [] => True
+        | b :: bs => wf_binder n b /\ go_list n bs
+        end
+    in
+    match e with
+    | var x => x < n
+    | op o bs => go_list n bs
+    end
+  with wf_binder (n : nat) (b : binder) :=
+         match b with
+         | bind s e => wf (s + n) e
+         end.
+  Definition wf_binders :=
+    fix go_list (n : nat) (bs : list binder) :=
+        match bs with
+        | [] => True
+        | b :: bs => wf_binder n b /\ go_list n bs
+        end.
+
+  Fixpoint shift (c d : nat) (e : t) : t :=
+    let fix go_list (c d : nat) (bs : list binder) : list binder :=
+        match bs with
+        | [] => []
+        | b :: bs => shift_binder c d b :: go_list c d bs
+        end
+    in
+        match e with
+        | var x => var (if x <? c then x else x + d)
+        | op o bs => op o (go_list c d bs)
+        end
+  with shift_binder (c d : nat) (b : binder) : binder :=
+         match b with
+         | bind n e => bind n (shift (n + c) d e)
+         end
+  .
+  Definition shift_binders :=
+    fix go_list (c d : nat) (bs : list binder) : list binder :=
+        match bs with
+        | [] => []
+        | b :: bs => shift_binder c d b :: go_list c d bs
+        end.
+
+  Fixpoint identity_subst (n : nat) : list t :=
+    match n with
+    | 0 => []
+    | S n => var 0 :: map (shift 0 1) (identity_subst n)
+    end.
+
+  Lemma identity_subst_length : forall n, length (identity_subst n) = n.
+  Proof.
+    induction n; simpl.
+    - auto.
+    - rewrite map_length. auto using f_equal.
+  Qed.
+  Hint Rewrite identity_subst_length : list.
+
+  Definition descend (n : nat) (rho : list t) : list t :=
+    (identity_subst n ++ map (shift 0 n) rho).
+
+  Lemma descend_length :
+    forall n rho,
+      length (descend n rho) = n + length rho.
+  Proof.
+    intros.
+    unfold descend.
+    now rewrite app_length, map_length, identity_subst_length.
+  Qed.
+
+  Fixpoint subst (rho : list t) (e : t) : t :=
+    let fix go_list (rho : list t) (bs : list binder) : list binder :=
+        match bs with
+        | [] => []
+        | b :: bs => subst_binder rho b :: go_list rho bs
+        end
+    in
+    match e with
+    | var x => match nth_error rho x with
+              | Some e' => e'
+              | None => e
+              end
+    | op o bs => op o (go_list rho bs)
+    end
+  with subst_binder (rho : list t) (b : binder) : binder :=
+         match b with
+         | bind n e => bind n (subst (descend n rho) e)
+         end
+  .
+  Definition subst_binders :=
+    fix go_list (rho : list t) (bs : list binder) : list binder :=
+        match bs with
+        | [] => []
+        | b :: bs => subst_binder rho b :: go_list rho bs
+        end.
+
+  Lemma shift_shift :
+    forall e c1 d1 c2 d2,
+      c2 <= c1 ->
+      shift c2 d2 (shift c1 d1 e) =
+      shift (c1 + d2) d1 (shift c2 d2 e).
+  Proof.
+    induction e using rect
+    with (Pb := fun b =>
+             forall c1 d1 c2 d2,
+               c2 <= c1 ->
+               shift_binder c2 d2 (shift_binder c1 d1 b) =
+               shift_binder (c1 + d2) d1 (shift_binder c2 d2 b))
+         (Pbl := fun bs =>
+             forall c1 d1 c2 d2,
+               c2 <= c1 ->
+               shift_binders c2 d2 (shift_binders c1 d1 bs) =
+               shift_binders (c1 + d2) d1 (shift_binders c2 d2 bs));
+      intros c1 d1 c2 d2 LE; simpl; f_equal; auto.
+    - repeat do_ltb; omega.
+    - simpl.
+      rewrite IHe by omega.
+      f_equal.
+      omega.
+  Qed.
+
+  Lemma shift_nop :
+    forall e c d n,
+      n <= c ->
+      wf n e ->
+      shift c d e = e.
+  Proof.
+    induction e using rect
+    with (Pb := fun b =>
+                  forall c d n,
+                    n <= c ->
+                    wf_binder n b ->
+                    shift_binder c d b = b)
+           (Pbl := fun bs =>
+                     forall c d n,
+                       n <= c ->
+                       wf_binders n bs ->
+                       shift_binders c d bs = bs);
+      simpl; intros c d n LE WF; f_equal; intuition eauto.
+    - destruct (Nat.ltb_spec x c); auto.
+      omega.
+    - eapply IHe; try eassumption. omega.
+  Qed.
+
+
+  Lemma shift_identity_subst :
+    forall n c d,
+      n <= c ->
+      map (shift c d) (identity_subst n) = identity_subst n.
+  Proof.
+    induction n; simpl; intros c d LE.
+    - reflexivity.
+    - f_equal.
+      + destruct (Nat.ltb_spec 0 c); auto.
+        omega.
+      + destruct c; [omega|].
+        rewrite <- IHn with (c := c) (d := d) at 2 by omega.
+        rewrite !map_map.
+        apply map_ext.
+        intros e.
+        rewrite shift_shift with (c2 := 0) by omega.
+        f_equal. omega.
+  Qed.
+
+  Lemma descend_shift :
+    forall n rho c d,
+      descend n (map (shift c d) rho) =
+      map (shift (n + c) d) (descend n rho).
+  Proof.
+    unfold descend.
+    intros.
+    rewrite map_app.
+    f_equal.
+    - now rewrite shift_identity_subst by omega.
+    - rewrite !map_map.
+      apply map_ext.
+      intros e.
+      rewrite shift_shift by omega.
+      f_equal.
+      omega.
+  Qed.
+
+  Hint Rewrite app_length nth_error_map : list.
+  Hint Rewrite map_app app_ass : list.
+
+  Lemma descend_app :
+    forall s rho1 rho2,
+      descend s (rho1 ++ rho2) = descend s rho1 ++ map (shift 0 s) rho2.
+  Proof.
+    intros.
+    unfold descend.
+    now autorewrite with list.
+  Qed.
+
+  Hint Rewrite descend_app descend_length : list.
+
+  Lemma shift_subst :
+    forall e c d rho,
+      wf (List.length rho) e ->
+      shift c d (subst rho e) =
+      subst (List.map (shift c d) rho) e.
+  Proof.
+    induction e using rect
+    with (Pb := fun b =>
+             forall c d rho,
+               wf_binder (List.length rho) b ->
+               shift_binder c d (subst_binder rho b) =
+               subst_binder (List.map (shift c d) rho) b)
+         (Pbl := fun bs =>
+             forall c d rho,
+               wf_binders (List.length rho) bs ->
+               shift_binders c d (subst_binders rho bs) =
+               subst_binders (List.map (shift c d) rho) bs);
+      simpl; intros c d rho WF; f_equal; intuition; autorewrite with list in *.
+    - break_match; auto.
+      do_nth_error_Some.
+      intuition omega.
+    - rewrite IHe by now rewrite descend_length.
+      f_equal.
+      now rewrite descend_shift.
+  Qed.
+
+
+  Lemma subst_shift :
+    forall e rho1 rho2 rho3,
+      wf (List.length (rho1 ++ rho3)) e ->
+      subst (rho1 ++ rho2 ++ rho3) (shift (List.length rho1) (List.length rho2) e) =
+      subst (rho1 ++ rho3) e.
+  Proof.
+    induction e using rect
+    with (Pb := fun b =>
+         forall rho1 rho2 rho3,
+           wf_binder (List.length (rho1 ++ rho3)) b ->
+           subst_binder (rho1 ++ rho2 ++ rho3)
+                        (shift_binder (List.length rho1) (List.length rho2) b) =
+           subst_binder (rho1 ++ rho3) b)
+         (Pbl := fun bs =>
+         forall rho1 rho2 rho3,
+           wf_binders (List.length (rho1 ++ rho3)) bs ->
+           subst_binders (rho1 ++ rho2 ++ rho3)
+                         (shift_binders (List.length rho1) (List.length rho2) bs) =
+           subst_binders (rho1 ++ rho3) bs);
+      simpl; intros rho1 rho2 rho3 WF; fold subst_binders shift_binders wf_binders in *;
+        f_equal; intuition; autorewrite with list in *.
+    - do_ltb.
+      + now rewrite !nth_error_app1 by assumption.
+      + rewrite !nth_error_app2 by omega.
+        do_app2_minus.
+        do_nth_error_Some.
+        break_match; intuition.
+    - erewrite <- IHe.
+      now f_equal; autorewrite with list.
+      now autorewrite with list; rewrite plus_assoc in *.
+  Qed.
+
+  Lemma subst_shift' :
+    forall e rho1 rho2,
+      wf (List.length rho2) e ->
+      subst (rho1 ++ rho2) (shift 0 (List.length rho1) e) =
+      subst rho2 e.
+  Proof.
+    intros.
+    now apply subst_shift with (rho1 := []).
+  Qed.
+
+  Lemma shift_nop_d :
+    forall e c,
+      shift c 0 e = e.
+  Proof.
+    induction e using rect
+    with (Pb := fun b =>
+             forall c,
+               shift_binder c 0 b = b)
+         (Pbl := fun bs =>
+             forall c,
+               shift_binders c 0 bs = bs);
+      simpl; intros c; fold subst_binders shift_binders wf_binders in *;
+        f_equal; intuition; autorewrite with list in *.
+    repeat do_ltb; omega.
+  Qed.
+
+  Local Notation SIS d n := (map (shift 0 d) (identity_subst n)).
+
+  Lemma shift_merge :
+    forall e c d1 d2,
+      shift c d2 (shift c d1 e) = shift c (d2 + d1) e.
+  Proof.
+    induction e using rect
+    with (Pb := fun b =>
+             forall c d1 d2,
+               shift_binder c d2 (shift_binder c d1 b) = shift_binder c (d2 + d1) b)
+         (Pbl := fun bs =>
+             forall c d1 d2,
+               shift_binders c d2 (shift_binders c d1 bs) = shift_binders c (d2 + d1) bs);
+      simpl; intros c d1 d2; fold subst_binders shift_binders wf_binders in *;
+        f_equal; intuition; autorewrite with list in *.
+    repeat do_ltb; omega.
+  Qed.
+
+  Lemma SIS_merge :
+    forall n d1 d2,
+      map (shift 0 d2) (SIS d1 n) = SIS (d1 + d2) n.
+  Proof.
+    intros.
+    rewrite !map_map.
+    apply map_ext.
+    intros e.
+    rewrite shift_merge.
+    f_equal.
+    omega.
+  Qed.
+
+  Lemma subst_identity_subst :
+    forall n rho1 rho2,
+      map (subst (rho1 ++ SIS (length rho1) n ++ rho2)) (SIS (length rho1) n) =
+      SIS (length rho1) n.
+  Proof.
+    induction n; simpl; intros rho1 rho2.
+    - reflexivity.
+    - f_equal.
+      + rewrite nth_error_app2 by omega.
+        now rewrite minus_diag.
+      + rewrite SIS_merge.
+        specialize (IHn (rho1 ++ [var (length rho1)]) rho2).
+        autorewrite with list in *.
+        simpl in *.
+        rewrite <- plus_n_Sm, <- plus_n_O in *.
+        assumption.
+  Qed.
+
+  Lemma SIS_0 :
+    forall n,
+      SIS 0 n = identity_subst n.
+  Proof.
+    intros.
+    erewrite map_ext.
+    now rewrite map_id.
+    intros e.
+    now rewrite shift_nop_d.
+  Qed.
+
+  Lemma descend_subst :
+    forall s rho1 rho2,
+      Forall (wf (length rho2)) rho1 ->
+      descend s (map (subst rho2) rho1) =
+      map (subst (descend s rho2)) (descend s rho1).
+  Proof.
+    intros s rho1 rho2 WF.
+    unfold descend.
+    autorewrite with list.
+    symmetry.
+    f_equal.
+    - generalize (map (shift 0 s) rho2). clear WF rho1 rho2. intro rho.
+      pose proof subst_identity_subst s [] rho.
+      simpl in *.
+      now rewrite SIS_0 in *.
+    - rewrite !map_map.
+      apply map_ext_in.
+      intros e I.
+      assert (wf (length rho2) e) by (eapply Forall_forall; eauto).
+      rewrite shift_subst by assumption.
+      pose proof subst_shift' e (identity_subst s) (map (shift 0 s) rho2).
+      autorewrite with list in *.
+      auto.
+  Qed.
+
+  Lemma wf_shift :
+    forall e c d n,
+      wf n e ->
+      wf (d + n) (shift c d e).
+  Proof.
+    induction e using rect
+    with (Pb := fun b =>
+             forall c d n,
+               wf_binder n b ->
+               wf_binder (d + n) (shift_binder c d b))
+         (Pbl := fun bs =>
+             forall c d n,
+               wf_binders n bs ->
+               wf_binders (d + n) (shift_binders c d bs));
+      simpl; intros c d n; fold subst_binders shift_binders wf_binders in *;
+        f_equal; intuition; autorewrite with list in *.
+    - do_ltb; omega.
+    - specialize (IHe (s + c) d (s + n)).
+      intuition.
+      now rewrite Nat.add_shuffle3.
+  Qed.
+
+  Lemma identity_subst_wf :
+    forall n,
+      Forall (wf n) (identity_subst n).
+  Proof.
+    induction n; simpl; constructor.
+    - simpl. omega.
+    - rewrite Forall_map. eapply Forall_impl; [|apply IHn].
+      intros ty WF.
+      now apply wf_shift with (c := 0) (d := 1).
+  Qed.
+
+  Lemma wf_weaken :
+    forall e n d,
+      n <= d ->
+      wf n e ->
+      wf d e.
+  Proof.
+    induction e using rect
+    with (Pb := fun b =>
+             forall n d,
+               n <= d ->
+               wf_binder n b ->
+               wf_binder d b)
+         (Pbl := fun bs =>
+             forall n d,
+               n <= d ->
+               wf_binders n bs ->
+               wf_binders d bs);
+      simpl; intros n d LE WF; fold subst_binders shift_binders wf_binders in *;
+        f_equal; intuition; autorewrite with list in *; eauto with arith.
+  Qed.
+
+  Lemma descend_wf :
+    forall n s rho,
+      Forall (wf n) rho ->
+      Forall (wf (s + n)) (descend s rho).
+  Proof.
+    intros n s rho WF.
+    unfold descend.
+    rewrite Forall_app.
+    split.
+    - eapply Forall_impl; [|apply identity_subst_wf].
+      eauto using wf_weaken with arith.
+    - rewrite Forall_map.
+      eapply Forall_impl; [|eassumption].
+      auto using wf_shift.
+  Qed.
+
+  Lemma wf_subst :
+    forall e n rho,
+      wf (length rho) e ->
+      List.Forall (wf n) rho ->
+      wf n (subst rho e).
+  Proof.
+    induction e using rect
+    with (Pb := fun b =>
+             forall n rho,
+               wf_binder (length rho) b ->
+               List.Forall (wf n) rho ->
+               wf_binder n (subst_binder rho b))
+         (Pbl := fun bs =>
+             forall n rho,
+               wf_binders (length rho) bs ->
+               List.Forall (wf n) rho ->
+               wf_binders n (subst_binders rho bs));
+      simpl; intros c d1 d2; fold subst_binders shift_binders wf_binders in *;
+        f_equal; intuition; autorewrite with list in *.
+    - break_match.
+      + eapply Forall_nth; eauto.
+      + do_nth_error_Some. intuition.
+    - apply IHe.
+      + now autorewrite with list.
+      + now apply descend_wf.
+  Qed.
+
+  Lemma subst_subst :
+    forall e rho1 rho2,
+      wf (List.length rho1) e ->
+      List.Forall (wf (List.length rho2)) rho1 ->
+      subst rho2 (subst rho1 e) =
+      subst (List.map (subst rho2) rho1) e.
+  Proof.
+    induction e using rect
+    with (Pb := fun b =>
+         forall rho1 rho2,
+           wf_binder (List.length rho1) b ->
+           List.Forall (wf (List.length rho2)) rho1 ->
+           subst_binder rho2 (subst_binder rho1 b) =
+           subst_binder (List.map (subst rho2) rho1) b)
+         (Pbl := fun bs =>
+         forall rho1 rho2,
+           wf_binders (List.length rho1) bs ->
+           List.Forall (wf (List.length rho2)) rho1 ->
+           subst_binders rho2 (subst_binders rho1 bs) =
+           subst_binders (List.map (subst rho2) rho1) bs);
+      simpl; intros rho1 rho2 rho3 WF; fold subst_binders shift_binders wf_binders in *;
+        autorewrite with list in *;
+        f_equal; intuition.
+    - break_match; auto.
+      do_nth_error_Some. intuition.
+    - rewrite IHe.
+      + f_equal. now rewrite descend_subst.
+      + now autorewrite with list.
+      + autorewrite with list.
+        auto using descend_wf.
+  Qed.
+
+  Lemma nth_error_identity_subst :
+    forall n x y,
+      nth_error (identity_subst n) x = Some y ->
+      y = var x.
+  Proof.
+    induction n; intros x y NE; destruct x; simpl in *; try congruence.
+    rewrite nth_error_map in NE.
+    break_match; try discriminate.
+    apply IHn in Heqo.
+    subst. simpl in *.
+    rewrite Nat.add_1_r in *.
+    congruence.
+  Qed.
+
+  Lemma SIS_unroll :
+    forall n d, SIS d (S n) = var d :: SIS (S d) n.
+  Proof.
+    intros.
+    simpl.
+    now rewrite SIS_merge.
+  Qed.
+  Lemma SIS_unroll_r :
+    forall n d, SIS d (S n) = SIS d n ++ [var (d + n)].
+  Proof.
+    induction n; intros.
+    - simpl. do 2 f_equal. omega.
+    - rewrite !SIS_unroll with (d := d).
+      rewrite IHn.
+      simpl.
+      repeat f_equal.
+      omega.
+  Qed.
+
+  Lemma identity_subst_unroll_r :
+    forall n,
+      identity_subst (S n) = identity_subst n ++ [var n].
+  Proof.
+    intros.
+    pose proof SIS_unroll_r n 0.
+    now rewrite !SIS_0 in *.
+  Qed.
+
+  Lemma descend_identity :
+    forall s n,
+      descend s (identity_subst n) = identity_subst (s + n).
+  Proof.
+    unfold descend.
+    intros s n.
+    rewrite plus_comm.
+    revert s.
+    induction n; simpl; intros s.
+    - now rewrite app_nil_r.
+    - rewrite SIS_merge.
+      specialize (IHn (S s)).
+      rewrite identity_subst_unroll_r in *.
+      rewrite app_ass in IHn.
+      cbn [app] in IHn.
+      cbn [plus].
+      rewrite IHn.
+      now rewrite <- plus_n_Sm.
+  Qed.
+
+  Lemma subst_identity :
+    forall e n,
+      subst (identity_subst n) e = e.
+  Proof.
+    induction e using rect
+    with (Pb := fun b =>
+            forall n,
+              subst_binder (identity_subst n) b = b)
+         (Pbl := fun bs =>
+            forall n,
+              subst_binders (identity_subst n) bs = bs);
+      simpl; intros n; fold subst_binders shift_binders wf_binders in *;
+        autorewrite with list in *;
+        f_equal; intuition.
+    - break_match; auto.
+      now apply nth_error_identity_subst in Heqo.
+    - rewrite descend_identity. auto.
+  Qed.
+
+  Lemma subst_empty :
+    forall e,
+      subst [] e = e.
+  Proof.
+    intros e.
+    exact (subst_identity e 0).
+  Qed.
+
+  Lemma subst_shift_cons :
+    forall e e' g,
+      wf (length g) e ->
+      subst (e' :: g) (shift 0 1 e) = subst g e.
+  Proof.
+    intros.
+    pose proof subst_shift e [] [e'] g.
+    auto.
+  Qed.
+
+  Lemma subst_shift_singleton :
+    forall e e',
+      wf 0 e ->
+      subst [e'] (shift 0 1 e) = e.
+  Proof.
+    intros.
+    rewrite subst_shift_cons by auto.
+    now rewrite subst_identity with (n := 0).
+  Qed.
+
+  Lemma descend_0 :
+    forall rho,
+      descend 0 rho = rho.
+  Proof.
+    unfold descend.
+    intros.
+    simpl.
+    erewrite map_ext, map_id; auto.
+    simpl.
+    intros e.
+    now rewrite shift_nop_d.
+  Qed.
+End abt.
+
